isabelle/examples/dynamic_logics/pdl.thy
@@ -1,16 +1,12 @@
-section \<open>Shallow Embedding of Propositional Dynamic Logic (PDL)\<close>
-
 theory pdl
   imports "../../operators" "../../entailment"
 begin
 
-
-typedecl w (*type of worlds or states*)
-type_synonym \<sigma> = "Set(w)" (*type of propositions or predicates*)
-type_synonym \<pi> = "ERel(w)" (*type of actions or programs*)
+section \<open>Shallow Embedding of Propositional Dynamic Logic (PDL)\<close>  (*Beware: work in progress!*)
 
 (*Syntactic sugar for object-logical Boolean connectives*)
 notation(input) compl ("\<^bold>\<not>") and inter (infixr "\<^bold>\<and>" 54) and union (infixr "\<^bold>\<or>" 53) and impl  (infixr "\<^bold>\<rightarrow>" 51)
+notation(input) emptyset ("\<^bold>\<bottom>") and universe ("\<^bold>\<top>")
 
 (*We now introduce our program-indexed family of modalities via the following definitions:*)
 notation(input) leftImage ("<_>_")
@@ -36,8 +32,8 @@ subsection \<open>Operations\<close>
   For instance actions/programs can be combined via a sequential or choice execution.*)
 
 (*Sequential execution 'a' followed by 'b'*)
-abbreviation(input) seq_composition::"\<pi> \<Rightarrow> \<pi> \<Rightarrow> \<pi>" (infixr "\<^bold>;" 75) (*note boldface*)
-  where "a \<^bold>; b \<equiv> b \<circ>\<^sup>r a"
+abbreviation(input) seq_composition (infixr "\<^bold>;" 75) (*note boldface*)
+  where "a \<^bold>; b \<equiv> a ;\<^sup>r b"
 
 lemma "[a\<^bold>;b]P = [a][b]P" (*sledgehammer*)
   by (simp add: B1_comb_def leftDualImage_hom_comp)
@@ -45,7 +41,7 @@ lemma "<a\<^bold>;b>P = <a><b>P"
   by (simp add: B1_comb_def leftImage_hom_comp)
 
 (*Choice: execute a or b (non-deterministically)*)
-abbreviation(input) choice::"\<pi> \<Rightarrow> \<pi> \<Rightarrow> \<pi>" (infixr "+" 75)
+abbreviation(input) choice (infixr "+" 75)
   where "a + b \<equiv> a \<union>\<^sup>r b"
 
 (*P holds in every state reachable via execution of the action/program 'a+b' if and only if P holds 
@@ -59,7 +55,7 @@ lemma "<a+b>P = (<a>P) \<^bold>\<or> (<b>P)"
   unfolding leftImage_def leftImage_hom_join rel_defs func_defs comb_defs by auto
 
 (*Non-deterministic choice for arbitrary sets: execute any action/program among those in S*)
-abbreviation(input) gen_choice::"Set(\<pi>) \<Rightarrow> \<pi>" ("\<Sigma>")
+abbreviation(input) gen_choice ("\<Sigma>")
   where "\<Sigma> S \<equiv> \<Union>\<^sup>rS" 
 
 lemma "[\<Sigma> S]P = \<Inter>\<lparr>(\<lambda>x. [x]P) S\<rparr>"
@@ -69,8 +65,8 @@ lemma "<\<Sigma> S>P = \<Union>\<lparr>(\<lambda>x. <x>P) S\<rparr>"
 
 (*Iterated execution ("Kleene star") corresponds to the (reflexive-)transitive closure of the 
  denotation of the program/action. It models "repeat an undetermined number of times". *)
-term "(\<lambda>a. a\<^sup>+) :: \<pi> \<Rightarrow> \<pi>"
-term "(\<lambda>a. a\<^sup>*) :: \<pi> \<Rightarrow> \<pi>"
+term "(\<lambda>a. a\<^sup>+) :: ERel('a) \<Rightarrow> ERel('a)"
+term "(\<lambda>a. a\<^sup>*) :: ERel('a) \<Rightarrow> ERel('a)"
 
 lemma tran_closure_refl: "reflexive R \<longrightarrow> reflexive (R\<^sup>+)"
   unfolding reflexive_def2  biginterR_def2 endorel_defs func_defs comb_defs rel_defs by blast
